theories/prepost.v
@@ -1,0 +1,166 @@
+Require Export refframe.module.
+Require Import refframe.trefines.
+Require Import refframe.link.
+Require Import refframe.seq_product.
+Require Import refframe.state_transform.
+Require Import refframe.proof_techniques.
+
+Set Default Proof Using "Type".
+
+(** * prepost *)
+Inductive prepost {R : Type} : Type :=
+| pp_end (r : R)
+| pp_prop (P : Prop) (pp : prepost)
+| pp_quant {T} (pp : T → prepost)
+.
+Arguments prepost : clear implicits.
+
+Fixpoint pp_to_ex {R} (pp : prepost R) (Q : R → Prop) : Prop :=
+  match pp with
+  | pp_end r => Q r
+  | pp_prop P pp' => P ∧ pp_to_ex pp' Q
+  | pp_quant pp' => ∃ x, pp_to_ex (pp' x) Q
+  end.
+
+Fixpoint pp_to_all {R} (pp : prepost R) (Q : R → Prop) : Prop :=
+  match pp with
+  | pp_end r => Q r
+  | pp_prop P pp' => P → pp_to_all pp' Q
+  | pp_quant pp' => ∀ x, pp_to_all (pp' x) Q
+  end.
+
+Lemma pp_to_ex_exists {R} pp Q:
+  @pp_to_ex R pp Q ↔ ∃ r, Q r ∧ pp_to_ex pp (r =.).
+Proof. elim: pp => /=; naive_solver. Qed.
+
+Lemma pp_to_all_ex {R} pp Q1 Q2:
+  @pp_to_all R pp Q1 →
+  pp_to_ex pp Q2 →
+  ∃ r, Q1 r ∧ Q2 r.
+Proof. elim: pp => /=; naive_solver. Qed.
+
+(** * mod_prepost *)
+Section prepost.
+  Context {EV1 EV2 S : Type}.
+  Implicit Types (i : EV2 → S → prepost (EV1 * S)) (o : EV1 → S → prepost (EV2 * S)).
+  Implicit Types (m : module EV1).
+
+  Inductive pp_state : Type :=
+  | PPOutside
+  | PPRecv1 (e : EV2)
+  | PPRecv2 (e : EV1)
+  | PPInside
+  | PPSend1 (e : EV1)
+  | PPSend2 (e : EV2)
+  .
+
+  Inductive pp_filter_step i o :
+    (pp_state * S) → option (EV1 + EV2) → ((pp_state * S) → Prop) → Prop :=
+  | PPOutsideS s e:
+    pp_filter_step i o (PPOutside, s) (Some (inr e)) (λ σ, σ = (PPRecv1 e, s))
+  | PPRecv1S s e:
+    pp_filter_step i o (PPRecv1 e, s) None (λ σ, pp_to_ex (i e s) (λ r, σ = (PPRecv2 r.1, r.2)))
+  | PPRecv2S s e:
+    pp_filter_step i o (PPRecv2 e, s) (Some (inl e)) (λ σ, σ = (PPInside, s))
+  | PPInsideS s e:
+    pp_filter_step i o (PPInside, s) (Some (inl e)) (λ σ, σ = (PPSend1 e, s))
+  | PPSend1S s e r:
+    pp_to_ex (o e s) (r=.) →
+    pp_filter_step i o (PPSend1 e, s) None (λ σ, σ = (PPSend2 r.1, r.2))
+  | PPSend2S s e:
+    pp_filter_step i o (PPSend2 e, s) (Some (inr e)) (λ σ, σ = (PPOutside, s))
+  .
+
+  Definition mod_prepost_filter i o :=
+    Mod (pp_filter_step i o).
+
+  Global Instance mod_prepost_filter_vis_no_all i o : VisNoAll (mod_prepost_filter i o).
+  Proof. move => ????. invert_all @m_step; naive_solver. Qed.
+
+  Definition mod_prepost i o m : module EV2 :=
+    mod_seq_map m (mod_prepost_filter i o).
+
+  Global Instance mod_prepost_vis_no_all i o m `{!VisNoAll m}: VisNoAll (mod_prepost i o m).
+  Proof. apply _. Qed.
+
+  Lemma mod_prepost_trefines i o m m' σ σ' σm s `{!VisNoAll m}:
+    trefines (MS m σ) (MS m' σ') →
+    trefines (MS (mod_prepost i o m) (σm, σ, s)) (MS (mod_prepost i o m') (σm, σ', s)).
+  Proof.
+    move => ?. apply mod_seq_map_trefines => //. apply _.
+  Qed.
+
+  Lemma mod_prepost_step_Outside_i i o m σ s:
+    TStepI (mod_prepost i o m) (SMFilter, σ, (PPOutside, s)) (λ G,
+        ∀ e, G true (Some e) (λ G', G' (SMFilter, σ, (PPRecv1 e, s)))).
+  Proof.
+    constructor => G /= ?. tstep_i.
+    apply steps_impl_step_end => ???. invert_all @m_step => ???. split! => ?. split!; [naive_solver|done|].
+    naive_solver.
+  Qed.
+
+  Lemma mod_prepost_step_Recv1_i i o m σ s e:
+    TStepI (mod_prepost i o m) (SMFilter, σ, (PPRecv1 e, s)) (λ G,
+        pp_to_ex (i e s) (λ r, G true None (λ G', G' (SMProgRecv r.1, σ, (PPInside, r.2))))).
+  Proof.
+    constructor => G /= /pp_to_ex_exists[r [HG Hex]]. tstep_i.
+    apply steps_impl_step_next => ???. invert_all @m_step.
+    eexists (_, _). split!. { apply pp_to_ex_exists. naive_solver. }
+    apply steps_impl_step_end => ???. invert_all @m_step => ???. naive_solver.
+  Qed.
+
+  Lemma mod_prepost_step_Inside_i i o m σ s e:
+    TStepI (mod_prepost i o m) (SMFilterRecv e, σ, (PPInside, s)) (λ G,
+        pp_to_all (o e s) (λ r, G true (Some (r.1)) (λ G', G' (SMFilter, σ, (PPOutside, r.2))))).
+  Proof.
+    constructor => G /= ?. apply steps_impl_step_trans. tstep_i.
+    apply steps_impl_step_end => ???. invert_all @m_step => ? b *; simplify_eq. split! => ?. split!; [done|].
+    tstep_i.
+    apply steps_impl_step_next => ???. invert_all @m_step => *; simplify_eq. split!.
+    apply steps_impl_step_end => ???. invert_all @m_step => *; simplify_eq. split! => ?.
+    have [?[??]]:= pp_to_all_ex _ _ _ ltac:(done) ltac:(done); subst.
+    split!; [done|by destruct b|]. naive_solver.
+  Qed.
+
+  Lemma mod_prepost_step_Outside_s i o m σ s:
+    TStepS (mod_prepost i o m) (SMFilter, σ, (PPOutside, s)) (λ G,
+        ∃ e, G (Some e) (λ G', G' (SMFilter, σ, (PPRecv1 e, s)))).
+  Proof.
+    constructor => G /= [??]. split!; [done|] => /= ??. tstep_s. eexists (Some (inr _)). split!; [done|].
+    apply: steps_spec_step_end; [by econs|]. naive_solver.
+  Qed.
+
+
+  Lemma mod_prepost_step_Recv1_s i o m σ s e:
+    TStepS (mod_prepost i o m) (SMFilter, σ, (PPRecv1 e, s)) (λ G,
+        G None (λ G', pp_to_all (i e s) (λ r, G' (SMProgRecv r.1, σ, (PPInside, r.2))))).
+  Proof.
+    constructor => G /= ?. split!; [done|] => /= ??. apply steps_spec_step_trans.
+    tstep_s. eexists None. split!.
+    apply: steps_spec_step_end; [by econs|] => ? /=?.
+    have [?[??]]:= pp_to_all_ex _ _ _ ltac:(done) ltac:(done); subst.
+    tstep_s. eexists (Some (inl _)). split!.
+    apply: steps_spec_step_end; [by econs|]. naive_solver.
+  Qed.
+
+  Lemma mod_prepost_step_Inside_s i o m σ s e:
+    TStepS (mod_prepost i o m) (SMFilterRecv e, σ, (PPInside, s)) (λ G,
+        pp_to_ex (o e s) (λ r, G (Some (r.1)) (λ G', G' (SMFilter, σ, (PPOutside, r.2))))).
+  Proof.
+    constructor => G /= /pp_to_ex_exists[?[??]]. split!; [done|] => /= ??.
+    apply steps_spec_step_trans. tstep_s. eexists (Some _). split!.
+    apply: steps_spec_step_end; [by econs|] => /= ? ->. tstep_s. eexists (Some (inr _)). split!; [done|].
+    apply: steps_spec_step; [by econs|] => /= ? ->.
+    apply: steps_spec_step_end; [by econs|] => /= ? ->.
+    done.
+  Qed.
+End prepost.
+
+Global Hint Resolve
+       mod_prepost_step_Outside_i
+       mod_prepost_step_Recv1_i
+       mod_prepost_step_Inside_i
+       mod_prepost_step_Outside_s
+       mod_prepost_step_Recv1_s
+       mod_prepost_step_Inside_s
+ | 3 : tstep.
